thys/Call_Arity/AnalBinds.thy
@@ -1,5 +1,5 @@
 theory AnalBinds
-imports Terms "HOLCF-Utils" Env
+imports "../Launchbury/Terms" "../Launchbury/HOLCF-Utils" "../Launchbury/Env"
 begin
 
 locale ExpAnalysis =
