thys/Call_Arity/CoCallGraph.thy
@@ -1,5 +1,5 @@
 theory CoCallGraph
-imports Main Vars "HOLCF-Join-Classes" "HOLCF-Utils" "Set-Cpo"
+imports "../Launchbury/Vars" "../Launchbury/HOLCF-Join-Classes" "../Launchbury/HOLCF-Utils" "Set-Cpo"
 begin
 
 default_sort type
