thys/Call_Arity/TransformTools.thy
@@ -1,5 +1,5 @@
 theory TransformTools
-imports "Nominal-HOLCF" Terms Substitution Env
+imports "../Launchbury/Nominal-HOLCF" "../Launchbury/Terms" "../Launchbury/Substitution" "../Launchbury/Env"
 begin
 
 default_sort type
