thys/Launchbury/Pointwise.thy
@@ -6,6 +6,6 @@ Lifting a relation to a function.
 
 definition pointwise where "pointwise P m m' = (\<forall> x. P (m x) (m' x))"
 
-lemma pointwiseI[intro]: "(\<And> x. P (m x) ( m' x)) \<Longrightarrow> pointwise P m m'" unfolding pointwise_def by blast
+lemma pointwiseI[intro]: "(\<And> x. P (m x) (m' x)) \<Longrightarrow> pointwise P m m'" unfolding pointwise_def by blast
 
 end
