thys/Launchbury/Substitution.thy
@@ -7,18 +7,6 @@ text {* Defining a substitution function on terms turned out to be slightly tric
 fun subst_var :: "var \<Rightarrow> var \<Rightarrow> var \<Rightarrow> var" ("_[_::v=_]" [1000,100,100] 1000)
   where "x[y ::v= z] = (if x = y then z else x)"
 
-(* Helper lemmas provided by Christian Urban *)
-
-lemma Projl_permute:
-  assumes a: "\<exists>y. f = Inl y"
-  shows "(p \<bullet> (Sum_Type.projl f)) = Sum_Type.projl (p \<bullet> f)"
-using a by auto
-
-lemma Projr_permute:
-  assumes a: "\<exists>y. f = Inr y"
-  shows "(p \<bullet> (Sum_Type.projr f)) = Sum_Type.projr (p \<bullet> f)"
-using a by auto
-
 nominal_function  (default "case_sum (\<lambda>x. Inl undefined) (\<lambda>x. Inr undefined)",
                   invariant "\<lambda> a r . (\<forall> as y z . ((a = Inr (as, y, z) \<and> atom ` domA as \<sharp>* (y, z)) \<longrightarrow> map (\<lambda>x . atom (fst x))  (Sum_Type.projr r) = map (\<lambda>x . atom (fst x)) as))")
   subst :: "exp \<Rightarrow> var \<Rightarrow> var \<Rightarrow> exp" ("_[_::=_]" [1000,100,100] 1000)
@@ -29,6 +17,8 @@ where
  |"(App e v)[y ::= z] = App (e[y ::= z]) (v[y ::v= z])"
  |"atom ` domA as \<sharp>* (y,z) \<Longrightarrow> (Let as body)[y ::= z] = Let (as[y ::h= z]) (body[y ::= z])" 
  |"atom x \<sharp> (y,z) \<Longrightarrow> (Lam [x].e)[y ::= z] = Lam [x].(e[y::=z])"
+ |"(Bool b)[y ::= z] = Bool b"
+ |"(scrut ? e1 : e2)[y ::= z] = (scrut[y ::= z] ? e1[y ::= z] : e2[y ::= z])"
  |"[][y ::h= z] = []"
  |"((v,e)# as)[y ::h= z] = (v, e[y ::= z])# (as[y ::h= z])"
 proof-
@@ -47,6 +37,16 @@ have eqvt_at_subst: "\<And> e y z . eqvt_at subst_subst_heap_sumC (Inl (e, y, z)
   apply simp
   apply(cases rule: subst_subst_heap_graph.cases)
   apply(assumption)
+  apply(rule_tac x="Sum_Type.projl x" in exI)
+  apply(clarify)
+  apply (rule the1_equality)
+  apply blast 
+  apply(simp (no_asm) only: sum.sel)
+  apply(rule_tac x="Sum_Type.projl x" in exI)
+  apply(clarify)
+  apply (rule the1_equality)
+  apply blast 
+  apply(simp (no_asm) only: sum.sel)
   apply(rule_tac x="Sum_Type.projl x" in exI)
   apply(clarify)
   apply (rule the1_equality)
@@ -137,7 +137,7 @@ next case (goal3 P x) show ?case
   qed
 qed
 
-next case (goal15 e y2 z2 as e2 y z as2) thus ?case
+next case (goal19 e y2 z2 as e2 y z as2) thus ?case
   apply -
   apply (drule eqvt_at_subst)+
   apply (drule eqvt_at_subst_heap)+
@@ -158,7 +158,7 @@ next case (goal15 e y2 z2 as e2 y z as2) thus ?case
   apply (simp add: eqvt_at_def)
   done
 
-next case (goal19 x2 y2 z2 e2 x y z e) thus ?case
+next case (goal25 x2 y2 z2 e2 x y z e) thus ?case
   apply -
   apply (drule eqvt_at_subst)+
   apply (simp only: Abs_fresh_iff meta_eq_to_obj_eq[OF subst_def, symmetric, unfolded fun_eq_iff])
@@ -179,6 +179,7 @@ lemma shows
 by(induct rule:subst_subst_heap.induct)
   (auto simp add: exp_assn.bn_defs fresh_star_insert)
 
+
 lemma subst_noop[simp]:
 shows "e[y ::= y] = e" and "as[y::h=y]= as"
 by(induct e y y and as y y rule:subst_subst_heap.induct)
@@ -192,7 +193,7 @@ and
  "atom ` domA as \<sharp>* y \<Longrightarrow> atom y \<sharp> as[y::h=z]"
 using assms
 by(induct e y z and as y z rule:subst_subst_heap.induct)
-  (auto simp add:fresh_at_base fresh_star_Pair fresh_star_insert fresh_Nil fresh_Cons)
+  (auto simp add:fresh_at_base fresh_star_Pair fresh_star_insert fresh_Nil fresh_Cons pure_fresh)
 
 lemma
  subst_pres_fresh: "x \<sharp> e \<Longrightarrow> x \<sharp> z \<Longrightarrow> x \<sharp> e[y ::= z]"
@@ -201,42 +202,90 @@ and
 by(induct e y z and \<Gamma> y z rule:subst_subst_heap.induct)
   (auto simp add:fresh_star_Pair exp_assn.bn_defs fresh_Cons)
 
+lemma subst_pres_fresh2:
+  "x \<sharp> y \<Longrightarrow> x \<sharp> z \<Longrightarrow> x \<sharp> e[y ::= z] \<longleftrightarrow> x \<sharp> e"
+and
+ "x \<sharp> y \<Longrightarrow> x \<sharp> z \<Longrightarrow> x \<notin> atom ` domA \<Gamma> \<Longrightarrow> x \<sharp> (\<Gamma>[y ::h= z]) \<longleftrightarrow> x \<sharp> \<Gamma>"
+by (induct e y z and \<Gamma> y z rule:subst_subst_heap.induct)
+   (auto simp add:fresh_star_Pair exp_assn.bn_defs fresh_Cons fresh_Pair)
+
 lemma subst_fresh_noop: "atom x \<sharp> e \<Longrightarrow> e[x ::= y] = e"
   and subst_heap_fresh_noop: "atom x \<sharp> \<Gamma> \<Longrightarrow>  \<Gamma>[x ::h= y] = \<Gamma>"
 by (nominal_induct  e and \<Gamma> avoiding: x y rule:exp_heap_strong_induct)
   (auto simp add: fresh_star_def fresh_Pair fresh_at_base fresh_Cons simp del: exp_assn.eq_iff)
 
-lemma supp_subst: "supp (e[y::=x]) \<subseteq> (supp e - {atom y}) \<union> supp x"
-proof-
-  have "\<And> a. (a \<sharp> e \<or> a = atom y) \<Longrightarrow> a \<sharp> x \<Longrightarrow> a \<sharp> e[y::=x]"
-    by (auto intro: subst_pres_fresh)
-  thus ?thesis by (auto simp add: fresh_def)
-qed
+lemma supp_subst_eq: "supp (e[y::=x]) = (supp e - {atom y}) \<union> (if atom y \<in> supp e then {atom x} else {})"
+  and  "atom ` domA \<Gamma> \<sharp>* y \<Longrightarrow> supp (\<Gamma>[y::h=x]) = (supp \<Gamma> - {atom y}) \<union> (if atom y \<in> supp \<Gamma> then {atom x} else {})"
+by (nominal_induct  e  and \<Gamma> avoiding: x y rule:exp_heap_strong_induct)
+   (auto simp add: fresh_star_def fresh_Pair supp_Nil supp_Cons supp_Pair fresh_Cons exp_assn.supp Let_supp supp_at_base pure_supp simp del: exp_assn.eq_iff)
+
+lemma supp_subst: "supp (e[y::=x]) \<subseteq> (supp e - {atom y}) \<union> {atom x}"
+  using supp_subst_eq by auto
+
+lemma fv_subst_eq: "fv (e[y::=x]) = (fv e - {y}) \<union> (if y \<in> fv e then {x} else {})"
+  and  "atom ` domA \<Gamma> \<sharp>* y \<Longrightarrow> fv (\<Gamma>[y::h=x]) = (fv \<Gamma> - {y}) \<union> (if y \<in> fv \<Gamma> then {x} else {})"
+by (nominal_induct  e  and \<Gamma> avoiding: x y rule:exp_heap_strong_induct)
+   (auto simp add: fresh_star_def fresh_Pair supp_Nil supp_Cons supp_Pair fresh_Cons exp_assn.supp Let_supp supp_at_base simp del: exp_assn.eq_iff)
 
 lemma fv_subst_subset: "fv (e[y ::= x]) \<subseteq> (fv e - {y}) \<union> {x}"
-proof-
-  have "fv (e[y ::= x]) = {v. atom v \<in> supp (e[y ::= x])}" unfolding fv_def..
-  also have "\<dots> \<subseteq> {v. atom v \<in> ((supp e - {atom y}) \<union> supp x)}"
-    using supp_subst by auto
-  also have "\<dots> = (fv e - {y}) \<union> {x}"
-    using supp_subst by (auto simp add: fv_def supp_at_base)
-  finally show ?thesis.
-qed
+  using fv_subst_eq by auto
 
-lemma fresh_star_at_base:
-  fixes x :: "'a :: at_base"
-  shows "S \<sharp>* x \<longleftrightarrow> atom x \<notin> S"
-  by (metis fresh_at_base(2) fresh_star_def)
+lemma fv_subst_int: "x \<notin> S \<Longrightarrow> y \<notin> S \<Longrightarrow> fv (e[y ::= x]) \<inter> S = fv e \<inter> S"
+  by (auto simp add: fv_subst_eq)
+
+lemma fv_subst_int2: "x \<notin> S \<Longrightarrow> y \<notin> S \<Longrightarrow> S \<inter> fv (e[y ::= x]) = S \<inter> fv e"
+  by (auto simp add: fv_subst_eq)
 
 lemma subst_swap_same: "atom x \<sharp> e \<Longrightarrow>  (x \<leftrightarrow> y) \<bullet> e = e[y ::=x]"
   and "atom x \<sharp> \<Gamma> \<Longrightarrow> atom `domA \<Gamma> \<sharp>* y \<Longrightarrow> (x \<leftrightarrow> y) \<bullet> \<Gamma> = \<Gamma>[y ::h= x]"
-by(nominal_induct  e and \<Gamma> avoiding: x y rule:exp_heap_strong_induct)
-  (auto simp add: fresh_star_Pair fresh_star_at_base fresh_Cons simp del: exp_assn.eq_iff)
+by (nominal_induct  e and \<Gamma> avoiding: x y rule:exp_heap_strong_induct)
+   (auto simp add: fresh_star_Pair fresh_star_at_base fresh_Cons pure_fresh permute_pure simp del: exp_assn.eq_iff)
 
 lemma subst_subst_back: "atom x \<sharp> e \<Longrightarrow>  e[y::=x][x::=y] = e" 
   and "atom x \<sharp> \<Gamma> \<Longrightarrow> atom `domA \<Gamma> \<sharp>* y  \<Longrightarrow> \<Gamma>[y::h=x][x::h=y] = \<Gamma>"
 by(nominal_induct  e and \<Gamma> avoiding: x y rule:exp_heap_strong_induct)
   (auto simp add: fresh_star_Pair fresh_star_at_base fresh_star_Cons fresh_Cons  exp_assn.bn_defs simp del: exp_assn.eq_iff)
 
+lemma subst_heap_delete[simp]: "(delete x \<Gamma>)[y ::h= z] = delete x (\<Gamma>[y ::h= z])"
+  by (induction \<Gamma>) auto
+
+lemma subst_nil_iff[simp]: "\<Gamma>[x ::h= z] = [] \<longleftrightarrow> \<Gamma> = []"
+  by (cases \<Gamma>) auto
+
+lemma subst_SmartLet[simp]:
+  "atom ` domA as \<sharp>* (y,z) \<Longrightarrow> (SmartLet as body)[y ::= z] = SmartLet (as[y ::h= z]) (body[y ::= z])"
+  unfolding SmartLet_def by auto
+
+lemma subst_let_be[simp]:
+  "atom x'  \<sharp> y \<Longrightarrow> atom x' \<sharp> x \<Longrightarrow> (let x' be e in exp )[y::=x] = (let x' be e[y::=x] in exp[y::=x])"
+  by (simp add: fresh_star_def fresh_Pair)
+
+lemma isLam_subst[simp]: "isLam e[x::=y] = isLam e"
+  by (nominal_induct e avoiding: x y  rule: exp_strong_induct)
+     (auto simp add: fresh_star_Pair)
+
+lemma isVal_subst[simp]: "isVal e[x::=y] = isVal e"
+  by (nominal_induct e avoiding: x y  rule: exp_strong_induct)
+     (auto simp add: fresh_star_Pair)
+
+lemma thunks_subst[simp]:
+  "thunks \<Gamma>[y::h=x] = thunks \<Gamma>"
+  by (induction \<Gamma>) (auto simp add: thunks_Cons)
+
+lemma map_of_subst:
+  "map_of (\<Gamma>[x::h=y]) k = map_option (\<lambda> e . e[x::=y]) (map_of \<Gamma> k)"
+by (induction \<Gamma> ) auto
+
+lemma mapCollect_subst[simp]:
+  "{e k v | k\<mapsto>v\<in>map_of \<Gamma>[x::h=y]} = {e k v[x::=y] | k\<mapsto>v\<in>map_of \<Gamma>}"
+  by (auto simp add: map_of_subst)
+
+lemma subst_eq_Cons:
+  "\<Gamma>[x::h=y] = (x', e)#\<Delta> \<longleftrightarrow> (\<exists> e' \<Gamma>'. \<Gamma> = (x',e')#\<Gamma>' \<and> e'[x::=y] = e \<and> \<Gamma>'[x::h=y] = \<Delta>)"
+  by (cases \<Gamma>) auto
+
+lemma nonrec_subst:
+  "atom ` domA \<Gamma> \<sharp>* x \<Longrightarrow> atom ` domA \<Gamma> \<sharp>* y \<Longrightarrow> nonrec \<Gamma>[x::h=y] \<longleftrightarrow> nonrec \<Gamma>"
+  by (auto simp add: nonrec_def  fresh_star_def subst_eq_Cons fv_subst_eq)
 
 end
