thys/Launchbury/Value.thy
@@ -1,10 +1,10 @@
 theory "Value"
-  imports HOLCF
+  imports "~~/src/HOL/HOLCF/HOLCF"
 begin
 
 subsubsection {* The semantic domain for values and environments *}
 
-domain Value = Fn (lazy "Value \<rightarrow> Value")
+domain Value = Fn (lazy "Value \<rightarrow> Value") | B (lazy "bool discr")
 
 fixrec Fn_project :: "Value \<rightarrow> Value \<rightarrow> Value"
  where "Fn_project\<cdot>(Fn\<cdot>f) = f"
@@ -12,17 +12,29 @@ fixrec Fn_project :: "Value \<rightarrow> Value \<rightarrow> Value"
 abbreviation Fn_project_abbr (infix "\<down>Fn" 55)
   where "f \<down>Fn v \<equiv> Fn_project\<cdot>f\<cdot>v"
 
-lemma [simp]: "\<bottom> \<down>Fn x = \<bottom>"
-  by (fixrec_simp)
+lemma [simp]:
+  "\<bottom> \<down>Fn x = \<bottom>"
+  "(B\<cdot>b) \<down>Fn x = \<bottom>"
+  by (fixrec_simp)+
+
+fixrec B_project :: "Value \<rightarrow> Value \<rightarrow> Value \<rightarrow> Value" where
+  "B_project\<cdot>(B\<cdot>db)\<cdot>v\<^sub>1\<cdot>v\<^sub>2 = (if undiscr db then v\<^sub>1 else v\<^sub>2)"
+
+lemma [simp]:
+  "B_project\<cdot>(B\<cdot>(Discr b))\<cdot>v\<^sub>1\<cdot>v\<^sub>2 = (if b then v\<^sub>1 else v\<^sub>2)"
+  "B_project\<cdot>\<bottom>\<cdot>v\<^sub>1\<cdot>v\<^sub>2 = \<bottom>"
+  "B_project\<cdot>(Fn\<cdot>f)\<cdot>v\<^sub>1\<cdot>v\<^sub>2 = \<bottom>"
+by fixrec_simp+
 
 text {*
 A chain in the domain @{typ Value} is either always bottom, or eventually @{term "Fn"} of another
 chain
 *}
 
-lemma Value_chainE:
+lemma Value_chainE[consumes 1, case_names bot B Fn]:
   assumes "chain Y"
   obtains "Y = (\<lambda> _ . \<bottom>)" |
+          n b where "Y = (\<lambda> m. (if m < n then \<bottom> else B\<cdot>b))" |
           n Y' where "Y = (\<lambda> m. (if m < n then \<bottom> else Fn\<cdot>(Y' (m-n))))" "chain Y'"
 proof(cases "Y = (\<lambda> _ . \<bottom>)")
   case True
@@ -33,22 +45,44 @@ next
   hence "\<exists> n. Y n \<noteq> \<bottom> \<and> (\<forall>m. Y m \<noteq> \<bottom> \<longrightarrow> m \<ge> n)"
     by (rule exE)(rule ex_has_least_nat)
   then obtain n where "Y n \<noteq> \<bottom>" and "\<forall>m. m < n \<longrightarrow> Y m = \<bottom>" by fastforce
-  then obtain f where "Y n = Fn \<cdot> f" by (metis Value.exhaust)
-  {
-    fix i
-    from `chain Y` have "Y n \<sqsubseteq> Y (i+n)" by (metis chain_mono le_add2)  
-    with `Y n = _`
-    have "\<exists> g. (Y (i+n) = Fn \<cdot> g)" by (metis (full_types) Value.exhaust minimal po_eq_conv)
-  }
-  then obtain Y' where Y': "\<And> i. Y (i + n) = Fn \<cdot> (Y' i)" by metis 
+  hence "(\<exists> f. Y n = Fn\<cdot>f) \<or> (\<exists> b. Y n = B\<cdot>b)" by (metis Value.exhaust)
+  thus ?thesis
+  proof
+    assume "(\<exists> f. Y n = Fn\<cdot>f)"
+    then obtain f where "Y n = Fn \<cdot> f" by blast
+    {
+      fix i
+      from `chain Y` have "Y n \<sqsubseteq> Y (i+n)" by (metis chain_mono le_add2)
+      with `Y n = _`
+      have "\<exists> g. (Y (i+n) = Fn \<cdot> g)"
+        by (metis Value.dist_les(1) Value.exhaust below_bottom_iff)
+    }
+    then obtain Y' where Y': "\<And> i. Y (i + n) = Fn \<cdot> (Y' i)" by metis
 
-  have "Y = (\<lambda>m. if m < n then \<bottom> else Fn\<cdot>(Y' (m - n)))"
-      using `\<forall>m. _` Y' by (metis add_diff_inverse add.commute)
-  moreover
-  have"chain Y'" using `chain Y`
-    by (auto intro!:chainI elim: chainE  simp add: Value.inverts[symmetric] Y'[symmetric] simp del: Value.inverts)
-  ultimately
-  show ?thesis by (rule that(2))
+    have "Y = (\<lambda>m. if m < n then \<bottom> else Fn\<cdot>(Y' (m - n)))"
+        using `\<forall>m. _` Y' by (metis add_diff_inverse add.commute)
+    moreover
+    have"chain Y'" using `chain Y`
+      by (auto intro!:chainI elim: chainE  simp add: Value.inverts[symmetric] Y'[symmetric] simp del: Value.inverts)
+    ultimately
+    show ?thesis by (rule that(3))
+  next
+    assume "(\<exists> b. Y n = B\<cdot>b)"
+    then obtain b where "Y n = B\<cdot>b" by blast
+    {
+      fix i
+      from `chain Y` have "Y n \<sqsubseteq> Y (i+n)" by (metis chain_mono le_add2)
+      with `Y n = _`
+      have "Y (i+n) = B\<cdot>b"
+        by (metis Value.dist_les(2) Value.exhaust Value.inverts(2) below_bottom_iff discrete_cpo)
+    }
+    hence  Y': "\<And> i. Y (i + n) = B\<cdot>b" by metis
+
+    have "Y = (\<lambda>m. if m < n then \<bottom> else B\<cdot>b)"
+        using `\<forall>m. _` Y' by (metis add_diff_inverse add.commute)
+    thus ?thesis by (rule that(2))
+  qed
 qed
+
 
 end
