thys/Launchbury/Vars.thy
@@ -1,4 +1,6 @@
-theory Vars imports Nominal2 begin
+theory Vars
+imports "../Nominal2/Nominal2"
+begin
 
 text {*
 The type of variables is abstract and provided by the Nominal package. All we know is that it is countable.
